current libs

specs/lib/fst/Spec.Lib.IntBuf.fst
@@ -29,9 +29,9 @@ let disjoint_list = admit()
 let create #a len init = Buf.create init (size_to_UInt32 len)
 let createL #a init = Buf.createL init
 
-let alloc #a #b len init read writes spec impl = 
+let alloc #a #b #len clen init read writes spec impl = 
   push_frame();
-  let buf = create len init in
+  let buf = create clen init in
   let r = impl buf in
   pop_frame();
   r
@@ -39,10 +39,18 @@ let alloc #a #b len init read writes spec impl =
 let index #a #len b i = Buf.index b (size_to_UInt32 i)
 let upd #a #len b i v = Buf.upd b (size_to_UInt32 i) v
 
-//let op_Array_Assignment = upd
-//let op_Array_Access = index
 
-let map #a #len f b = admit()
+let map #a #len clen f b = 
+  let h0 = ST.get() in
+  let inv (h1:mem) (j:nat) = True in
+  let f' (j:size_t{0 <= v j /\ v j <= len}) : Stack unit
+      (requires (fun h -> inv h (v j)))
+      (ensures (fun h1 _ h2 -> inv h2 (v j + 1))) = 
+      let b_i = b.(j) in
+      b.(j) <- f b_i in
+  Spec.Lib.Loops.for (size 0) clen inv f'
+
+
 let map2 #a1 #a2 #len clen f b1 b2 = 
   let h0 = ST.get() in
   let inv (h1:mem) (j:nat) = True in
@@ -53,8 +61,6 @@ let map2 #a1 #a2 #len clen f b1 b2 =
       let i2 = b2.(j) in
       b1.(j) <- f i1 i2 in
   Spec.Lib.Loops.for (size 0) clen inv f'
-
-let blit #a #len i start1 o start2 num = admit()
 
 let copy #a #len clen i o =
   let h0 = ST.get() in
@@ -70,9 +76,17 @@ let copy #a #len clen i o =
       o.(j) <- src_i in
   Spec.Lib.Loops.for (size 0) clen inv f'
 
-let repeat #a #b #lift n spec impl input = admit()
-let repeat_range #a #b #lift start fin spec impl input = admit()
-let repeati #a #b #lift fin spec impl input = admit()
+let iter_range #a #len start fin spec impl input = 
+  let h0 = ST.get() in
+  let inv (h1:mem) (j:nat) = True in
+  let f' (j:size_t{v start <= v j /\ v j <= v fin}) : Stack unit
+      (requires (fun h -> inv h (v j)))
+      (ensures (fun h1 _ h2 -> inv h2 (v j + 1))) = 
+      impl j input in
+  Spec.Lib.Loops.for start fin inv f'
+
+let iteri #a #len n spec impl input = iter_range #a #len (size 0) n spec impl input
+
 let iter #a #len n spec impl input = 
   let h0 = ST.get() in
   let inv (h1:mem) (j:nat) = True in
@@ -82,6 +96,3 @@ let iter #a #len n spec impl input =
       impl input in
   Spec.Lib.Loops.for (size 0) n inv f'
 
-
-let iteri #a #len n spec impl input = admit()
-let iter_range #a #len start fin spec impl input = admit()
