specs/lib/Spec.Lib.IntBuf.fsti
@@ -54,11 +54,11 @@ inline_for_extraction val createL: #a:Type0 -> init:list a{List.Tot.length init 
 				          /\ modifies1 r h0 h1 
 					  /\ as_lseq r h1 == LSeq.createL #a init))
 
-inline_for_extraction val alloc: #a:Type0 -> #b:Type0 -> len:size_t -> init:a -> 
+inline_for_extraction val alloc: #a:Type0 -> #b:Type0 -> #len:size_nat -> clen:size_t{v clen == len} -> init:a -> 
 		 reads:list bufitem ->
 		 writes:list bufitem ->
 		 spec:(h0:mem -> r:b -> h1:mem -> Type) ->
-		 impl:(buf:lbuffer a (v len) -> Stack b
+		 impl:(buf:lbuffer a len -> Stack b
 			   (requires (fun h -> live h buf /\ live_list h reads /\ live_list h writes /\ disjoint_list buf reads /\ disjoint_list buf writes))
 			   (ensures (fun h0 r h1 -> preserves_live h0 h1 /\
 						 modifies (BufItem buf :: writes) h0 h1 /\
@@ -82,7 +82,7 @@ inline_for_extraction val upd: #a:Type0 -> #len:size_nat -> b:lbuffer a (len) ->
 inline_for_extraction let op_Array_Assignment = upd
 inline_for_extraction let op_Array_Access = index
 
-val map: #a:Type -> #len:size_nat -> f:(a -> Tot a) -> b:lbuffer a (len) -> Stack unit 
+val map: #a:Type -> #len:size_nat -> clen:size_t{v clen == len} -> f:(a -> Tot a) -> b:lbuffer a (len) -> Stack unit 
 		      (requires (fun h0 -> live h0 b))
 		      (ensures (fun h0 _ h1 -> preserves_live h0 h1 /\ modifies1 b h0 h1 
 				  /\ as_lseq #a #len b h1 == LSeq.map #a #a #(len) f (as_lseq #a #len b h0)))
@@ -92,18 +92,6 @@ val map2: #a1:Type -> #a2:Type -> #len:size_nat -> clen:size_t{v clen == len} ->
 		      (requires (fun h0 -> live h0 b1 /\ live h0 b2))
 		      (ensures (fun h0 _ h1 -> preserves_live h0 h1 /\ modifies1 b1 h0 h1 /\ as_lseq #a1 #len b1 h1 == LSeq.map2 #a1 #a2 #a1 #len f (as_lseq #a1 #len b1 h0) (as_lseq #a2 #len b2 h0)))
 
-val blit: #a:Type -> #len:size_nat -> i:lbuffer a (len) -> start1:size_t -> 
-          o:lbuffer a (len) -> start2:size_t -> 
-	  num:size_t{v start1 + v num <=  len /\ v start2 + v num <= len} -> 
-	  Stack unit 
- 		  (requires (fun h0 -> live h0 i /\ live h0 o ))
-  		  (ensures (fun h0 _ h1 -> preserves_live h0 h1 /\ 
-		  			modifies1 o h0 h1 /\ 
-					as_lseq o h1 == 
-					   LSeq.update_sub (as_lseq o h0) 
-						(v start1) (v num)
-						(LSeq.sub (as_lseq i h0) (v start2) (v num))))
-
 inline_for_extraction
 val copy: #a:Type -> #len:size_nat -> clen:size_t{v clen == len} -> i:lbuffer a len -> o:lbuffer a len -> Stack unit 
  		  (requires (fun h0 -> live h0 i /\ live h0 o ))
@@ -112,6 +100,49 @@ val copy: #a:Type -> #len:size_nat -> clen:size_t{v clen == len} -> i:lbuffer a 
 					as_lseq o h1 == as_lseq i h0))
 
 
+inline_for_extraction
+val iter_range: #a:Type -> #len:size_nat -> start:size_t -> fin:size_t{v start <= v fin} ->
+         spec:(i:size_nat{v start <= i /\ i < v fin}  -> LSeq.lseq a (len) -> Tot (LSeq.lseq a (len))) -> 
+         impl:(i:size_t{v start <= v i /\ v i < v fin}  -> x:lbuffer a (len) -> Stack unit 
+			(requires (fun h0 -> live h0 x))
+			(ensures (fun h0 _ h1 -> preserves_live h0 h1 /\ 
+				              modifies1 x h0 h1 /\
+					      as_lseq #a #len x h1 == spec (v i) (as_lseq #a #len x h0)))) ->
+	    input:lbuffer a (len) ->
+	    Stack unit
+	    (requires (fun h0 -> live h0 input))
+	    (ensures (fun h0 _ h1 -> preserves_live h0 h1 /\ modifies1 input h0 h1 /\
+				  as_lseq #a #len input h1 ==  LSeq.repeat_range (v start) (v fin) spec (as_lseq #a #len input h0)))
+
+inline_for_extraction
+val iteri: #a:Type -> #len:size_nat -> n:size_t -> spec:(i:size_nat{i < v n}  -> LSeq.lseq a (len) -> Tot (LSeq.lseq a (len))) -> 
+         impl:(i:size_t{v i < v n}  -> x:lbuffer a (len) -> Stack unit 
+			(requires (fun h0 -> live h0 x))
+			(ensures (fun h0 _ h1 -> preserves_live h0 h1 /\ 
+				              modifies1 x h0 h1 /\
+					      as_lseq #a #len x h1 == spec (v i) (as_lseq #a #len x h0)))) ->
+	    input:lbuffer a (len) ->
+	    Stack unit
+	    (requires (fun h0 -> live h0 input))
+	    (ensures (fun h0 _ h1 -> preserves_live h0 h1 /\ modifies1 input h0 h1 /\
+				  as_lseq #a #len input h1 ==  LSeq.repeati (v n) spec (as_lseq #a #len input h0)))
+
+inline_for_extraction
+val iter: #a:Type -> #len:size_nat -> n:size_t -> spec:(LSeq.lseq a (len) -> LSeq.lseq a (len)) -> 
+         impl:(x:lbuffer a (len) -> Stack unit 
+			(requires (fun h0 -> live h0 x))
+			(ensures (fun h0 _ h1 -> preserves_live h0 h1 /\ 
+				              modifies1 x h0 h1 /\
+					      as_lseq #a #len x h1 == spec (as_lseq #a #len x h0)))) ->
+	    input:lbuffer a (len) ->
+	    Stack unit
+	    (requires (fun h0 -> live h0 input))
+	    (ensures (fun h0 _ h1 -> preserves_live h0 h1 /\ modifies1 input h0 h1 /\
+				  as_lseq #a #len input h1 ==  LSeq.repeat (v n) spec (as_lseq #a #len input h0)))
+
+
+
+(*
 val repeat: #a:Type -> #b:Type -> #lift:(mem -> b -> GTot (option a)) -> 
 	    n:size_t -> spec:(a -> Tot a) -> 
 	    impl:(x:b -> Stack unit (requires (fun h0 -> Some? (lift h0 x))) (ensures (fun h0 _ h1 -> Some? (lift h0 x) /\ Some? (lift h1 x) /\ Some?.v (lift h1 x) == spec (Some?.v (lift h0 x))))) ->
@@ -145,43 +176,5 @@ val repeati: #a:Type -> #b:Type -> #lift:(mem -> b -> GTot (option a)) ->
 	    (requires (fun h0 -> Some? (lift h0 input)))
 	    (ensures (fun h0 _ h1 -> Some? (lift h0 input) /\ Some? (lift h1 input) /\
 				  Some?.v (lift h1 input) ==  LSeq.repeati (v n) spec (Some?.v (lift h0 input))))
-				  
-inline_for_extraction
-val iter: #a:Type -> #len:size_nat -> n:size_t -> spec:(LSeq.lseq a (len) -> LSeq.lseq a (len)) -> 
-         impl:(x:lbuffer a (len) -> Stack unit 
-			(requires (fun h0 -> live h0 x))
-			(ensures (fun h0 _ h1 -> preserves_live h0 h1 /\ 
-				              modifies1 x h0 h1 /\
-					      as_lseq #a #len x h1 == spec (as_lseq #a #len x h0)))) ->
-	    input:lbuffer a (len) ->
-	    Stack unit
-	    (requires (fun h0 -> live h0 input))
-	    (ensures (fun h0 _ h1 -> preserves_live h0 h1 /\ modifies1 input h0 h1 /\
-				  as_lseq #a #len input h1 ==  LSeq.repeat (v n) spec (as_lseq #a #len input h0)))
 
-val iteri: #a:Type -> #len:size_nat -> n:size_t -> spec:(i:size_nat{i < v n}  -> LSeq.lseq a (len) -> Tot (LSeq.lseq a (len))) -> 
-         impl:(i:size_t{v i < v n}  -> x:lbuffer a (len) -> Stack unit 
-			(requires (fun h0 -> live h0 x))
-			(ensures (fun h0 _ h1 -> preserves_live h0 h1 /\ 
-				              modifies1 x h0 h1 /\
-					      as_lseq #a #len x h1 == spec (v i) (as_lseq #a #len x h0)))) ->
-	    input:lbuffer a (len) ->
-	    Stack unit
-	    (requires (fun h0 -> live h0 input))
-	    (ensures (fun h0 _ h1 -> preserves_live h0 h1 /\ modifies1 input h0 h1 /\
-				  as_lseq #a #len input h1 ==  LSeq.repeati (v n) spec (as_lseq #a #len input h0)))
-
-val iter_range: #a:Type -> #len:size_nat -> start:size_t -> fin:size_t{v start <= v fin} ->
-         spec:(i:size_nat{v start <= i /\ i < v fin}  -> LSeq.lseq a (len) -> Tot (LSeq.lseq a (len))) -> 
-         impl:(i:size_t{v start <= v i /\ v i < v fin}  -> x:lbuffer a (len) -> Stack unit 
-			(requires (fun h0 -> live h0 x))
-			(ensures (fun h0 _ h1 -> preserves_live h0 h1 /\ 
-				              modifies1 x h0 h1 /\
-					      as_lseq #a #len x h1 == spec (v i) (as_lseq #a #len x h0)))) ->
-	    input:lbuffer a (len) ->
-	    Stack unit
-	    (requires (fun h0 -> live h0 input))
-	    (ensures (fun h0 _ h1 -> preserves_live h0 h1 /\ modifies1 input h0 h1 /\
-				  as_lseq #a #len input h1 ==  LSeq.repeat_range (v start) (v fin) spec (as_lseq #a #len input h0)))
-
-
+*)
